PhysLean/StringTheory/FTheory/SU5U1/Potential/ChargeProfile/Irreducible/Completenss.lean
@@ -1,0 +1,622 @@
+/-
+Copyright (c) 2025 Joseph Tooby-Smith. All rights reserved.
+Released under Apache 2.0 license as described in the file LICENSE.
+Authors: Joseph Tooby-Smith
+-/
+import PhysLean.StringTheory.FTheory.SU5U1.Potential.ChargeProfile.Irreducible.Elems
+
+namespace FTheory
+
+namespace SU5U1
+
+variable {I : CodimensionOneConfig}
+namespace PotentialTerm
+
+namespace ChargeProfile
+
+
+/-!
+
+## Auxillary results: Multisets from Finsets of given cardinality.
+
+-/
+
+def toMultisetsOne (s : Finset ℤ) : Multiset (Multiset ℤ) :=
+  let X1 := (s.powersetCard 1).val.map fun X => X.val
+  X1
+
+@[simp]
+lemma mem_toMultisetsOne_iff {s : Finset ℤ} (X : Multiset ℤ) :
+    X ∈ toMultisetsOne s ↔ X.toFinset ⊆ s ∧ X.card = 1 := by
+  simp [toMultisetsOne]
+  intro h
+  rw [Multiset.card_eq_one] at h
+  obtain ⟨x, h1, h2⟩ := h
+  simp
+
+def toMultisetsTwo (s : Finset ℤ) : Multiset (Multiset ℤ) :=
+  let X1 := (s.powersetCard 1).val.map (fun X => X.val.bind (fun x => Multiset.replicate 2 x))
+  let X2 := (s.powersetCard 2).val.map fun X => X.val
+  X1 + X2
+
+@[simp]
+lemma mem_toMultisetsTwo_iff {s : Finset ℤ} (X : Multiset ℤ) :
+    X ∈ toMultisetsTwo s ↔ X.toFinset ⊆ s ∧ X.card = 2 := by
+  simp [toMultisetsTwo]
+  constructor
+  · intro h
+    rcases h with ⟨a, ⟨hasub, hacard⟩, hbind⟩ | ⟨h1, hcard⟩
+    · rw [Finset.card_eq_one] at hacard
+      obtain ⟨a, rfl⟩ := hacard
+      simp at hbind
+      subst hbind
+      simpa using hasub
+    · simp_all only [and_true]
+      refine Finset.subset_def.mpr ?_
+      simp only [Multiset.toFinset_val, Multiset.dedup_subset']
+      exact Multiset.subset_of_le h1
+  · intro ⟨hsub, hcard⟩
+    simp_all
+    rw [Multiset.card_eq_two] at hcard
+    obtain ⟨a, b, rfl⟩ := hcard
+    by_cases hab : a = b
+    · subst hab
+      left
+      use {a}
+      simpa using hsub
+    · right
+      refine (Multiset.le_iff_subset ?_).mpr ?_
+      · simpa using hab
+      · exact Multiset.dedup_subset'.mp hsub
+
+def toMultisetsThree (s : Finset ℤ) : Multiset (Multiset ℤ) :=
+  let X1 := (s.powersetCard 1).val.map (fun X => X.val.bind (fun x => Multiset.replicate 3 x))
+  let X2 := s.val.bind (fun x => (s \ {x}).val.map (fun y => {x} + Multiset.replicate 2 y))
+  let X3 := (s.powersetCard 3).val.map fun X => X.val
+  X1 + X2 + X3
+
+@[simp]
+lemma mem_toMultisetsThree_iff {s : Finset ℤ} (X : Multiset ℤ) :
+    X ∈ toMultisetsThree s ↔ X.toFinset ⊆ s ∧ X.card = 3 := by
+  simp [toMultisetsThree]
+  constructor
+  · intro h
+    rw [or_assoc] at h
+    rcases h with ⟨a, ⟨hasub, hacard⟩, hbind⟩ | ⟨a, ha, ⟨b, hb, rfl⟩⟩ | ⟨h1, hcard⟩
+    · rw [Finset.card_eq_one] at hacard
+      obtain ⟨a, rfl⟩ := hacard
+      simp at hbind
+      subst hbind
+      simpa using hasub
+    · simp only [Multiset.toFinset_cons, Multiset.toFinset_singleton, Finset.mem_insert,
+      Finset.mem_singleton, or_true, Finset.insert_eq_of_mem, Multiset.card_cons,
+      Multiset.card_singleton, Nat.reduceAdd, and_true]
+      refine Finset.insert_subset ha ?_
+      rw [← @Multiset.mem_toFinset] at hb
+      simp at hb
+      simp only [Finset.singleton_subset_iff]
+      exact Finset.mem_of_mem_erase hb
+    · simp_all only [and_true]
+      refine Finset.subset_def.mpr ?_
+      simp only [Multiset.toFinset_val, Multiset.dedup_subset']
+      exact Multiset.subset_of_le h1
+  · intro ⟨hsub, hcard⟩
+    simp_all
+    rw [Multiset.card_eq_three] at hcard
+    obtain ⟨a, b, c, rfl⟩ := hcard
+    by_cases hab : a = b
+    · subst hab
+      left
+      by_cases hac : a = c
+      · subst hac
+        left
+        use {a}
+        simpa using hsub
+      · right
+        simp [@Finset.insert_subset_iff] at hsub
+        use c
+        simp_all
+        use a
+        apply And.intro
+        · refine (Multiset.mem_erase_of_ne hac).mpr ?_
+          simp_all
+        · simp
+          rw [← Multiset.insert_eq_cons, Multiset.pair_comm c a]
+          simp
+    · rw [or_assoc]
+      right
+      by_cases hac : a = c
+      · subst hac
+        simp [@Finset.insert_subset_iff] at hsub
+        left
+        use b
+        simp_all
+        use a
+        simp
+        refine (Multiset.mem_erase_of_ne (by omega)).mpr ?_
+        simp_all
+      · by_cases hbc : b = c
+        · subst hbc
+          left
+          simp [@Finset.insert_subset_iff] at hsub
+          use a
+          simp_all
+          use b
+          apply And.intro
+          · refine (Multiset.mem_erase_of_ne (by omega)).mpr ?_
+            simp_all
+          exact Multiset.cons_swap b a {b}
+        · right
+          refine (Multiset.le_iff_subset ?_).mpr ?_
+          · simp
+            omega
+          · exact Multiset.dedup_subset'.mp hsub
+
+/-!
+
+## irreducibleSet'
+
+-/
+
+def irreducibleSet' (I : CodimensionOneConfig) : (T : PotentialTerm) → Multiset T.ChargeProfile
+  | μ =>
+    let SqHd := I.allowedBarFiveCharges.val
+    let SqHu := I.allowedBarFiveCharges.val
+    let prod := SqHd.product (SqHu)
+    let Filt := prod.filter (fun x => - x.1 + x.2 = 0)
+    (Filt.map (fun x => (x.1, x.2)))
+  | K2 =>
+    let SqHd := I.allowedBarFiveCharges.val
+    let SqHu := I.allowedBarFiveCharges.val
+    let Q10 := toMultisetsOne I.allowedTenCharges
+    let prod := SqHd.product (SqHu.product Q10)
+    let Filt := prod.filter (fun x => x.1 + x.2.1 + x.2.2.sum = 0)
+    (Filt.map (fun x => (x.1, x.2.1, x.2.2.toFinset)))
+  | K1 =>
+    let Q5 := toMultisetsOne I.allowedBarFiveCharges
+    let Q10 := toMultisetsTwo I.allowedTenCharges
+    let Prod := Q5.product Q10
+    let Filt := Prod.filter (fun x => - x.1.sum + x.2.sum = 0)
+    (Filt.map (fun x => (x.1.toFinset, x.2.toFinset)))
+  | W4 =>
+    let SqHd := I.allowedBarFiveCharges.val
+    let SqHu := I.allowedBarFiveCharges.val
+    let Q5 := toMultisetsOne I.allowedBarFiveCharges
+    let prod := SqHd.product (SqHu.product Q5)
+    let Filt := prod.filter (fun x => x.1 - 2 * x.2.1 + x.2.2.sum = 0)
+    (Filt.map (fun x => (x.1, x.2.1, x.2.2.toFinset)))
+  | W3 =>
+    let SqHu := I.allowedBarFiveCharges.val
+    let Q5 := toMultisetsTwo I.allowedBarFiveCharges
+    let prod := SqHu.product Q5
+    let Filt := prod.filter (fun x => - 2 * x.1 + x.2.sum = 0)
+    (Filt.map (fun x => (x.1, x.2.toFinset)))
+  | W2 =>
+    let SqHd := I.allowedBarFiveCharges.val
+    let Q10 := toMultisetsThree I.allowedTenCharges
+    let prod := SqHd.product Q10
+    let Filt := prod.filter (fun x => x.1 + x.2.sum = 0)
+    (Filt.map (fun x => (x.1, x.2.toFinset))).filter fun x => IsIrreducible x
+  | W1 =>
+    let Q5 := toMultisetsOne I.allowedBarFiveCharges
+    let Q10 := toMultisetsThree I.allowedTenCharges
+    let Prod := Q5.product Q10
+    let Filt := Prod.filter (fun x => x.1.sum + x.2.sum = 0)
+    (Filt.map (fun x => (x.1.toFinset, x.2.toFinset))).filter fun x => IsIrreducible x
+  | Λ =>
+    let Q5 := toMultisetsTwo I.allowedBarFiveCharges
+    let Q10 := toMultisetsOne I.allowedTenCharges
+    let Prod := Q5.product Q10
+    let Filt := Prod.filter (fun x => x.1.sum + x.2.sum = 0)
+    (Filt.map (fun x => (x.1.toFinset, x.2.toFinset)))
+  | β =>
+    let SqHu := I.allowedBarFiveCharges.val
+    let Q5 := toMultisetsOne I.allowedBarFiveCharges
+    let prod := SqHu.product Q5
+    let Filt := prod.filter (fun x => - x.1 + x.2.sum = 0)
+    (Filt.map (fun x => (x.1, x.2.toFinset)))
+  | topYukawa =>
+    let SqHu := I.allowedBarFiveCharges.val
+    let Q10 := toMultisetsTwo I.allowedTenCharges
+    let prod := SqHu.product Q10
+    let Filt := prod.filter (fun x => - x.1 + x.2.sum = 0)
+    (Filt.map (fun x => (x.1, x.2.toFinset)))
+  | bottomYukawa =>
+    let SqHd := I.allowedBarFiveCharges.val
+    let Q5 := toMultisetsOne I.allowedBarFiveCharges
+    let Q10 := toMultisetsOne I.allowedTenCharges
+    let prod := SqHd.product (Q5.product Q10)
+    let Filt := prod.filter (fun x => x.1 + x.2.1.sum + x.2.2.sum = 0)
+    (Filt.map (fun x => (x.1, x.2.1.toFinset, x.2.2.toFinset)))
+
+lemma irreducibleSet'_card_eq (I : CodimensionOneConfig) (T : PotentialTerm) :
+    (irreducibleSet' I T).card = irreducibleElemsCard I T := by
+  revert I T
+  decide
+
+lemma mem_irreducibleSet'_of_irreducible {I : CodimensionOneConfig} {T : PotentialTerm}
+    (x : ChargeProfile T) (h : IsIrreducible x) (hx : x ∈ finsetOfCodimensionOneConfig I T) :
+    x ∈ irreducibleSet' I T := by
+  match T, x with
+  | μ, (qHd, qHu) =>
+    simp [irreducibleSet']
+    have x_isPresent := isPresent_of_isIrreducible h
+    simp only [IsPresent, charges, Finset.product_eq_sprod, Multiset.mem_map, Prod.exists] at x_isPresent
+    simp only [← Multiset.mem_toFinset, Finset.val_toFinset, Finset.mem_product] at x_isPresent
+    obtain ⟨q1, q2, ⟨h1, h2⟩, hsum⟩ := x_isPresent
+    refine ⟨q1, q2, ⟨?_, ?_⟩, (h _ ?_).mpr ?_⟩
+    · -- membership of Multiset
+      rw [Option.mem_toFinset, Option.mem_def] at h1 h2
+      subst h1 h2
+      rw [finsetOfCodimensionOneConfig, Finset.product_eq_sprod, Finset.mem_product] at hx
+      simpa using hx
+    · -- sum
+      omega
+    · -- mem powerset
+      apply subset_of_iff_mem_powerset.mp
+      simp_all [Subset]
+    · -- is present
+      simp only [IsPresent, charges, Finset.product_eq_sprod, Multiset.mem_map, Prod.exists]
+      use q1, q2
+      simp only [Finset.singleton_product, Finset.map_val, Finset.product_val,
+        Finset.singleton_val, Function.Embedding.coeFn_mk, Multiset.mem_map,
+        Prod.mk.injEq, true_and, exists_eq_right]
+      repeat rw [SProd.sprod]
+      simp only [Multiset.instSProd]
+      rw [Multiset.mem_product]
+      simp only [Option.toFinset_some, Finset.singleton_val, Multiset.mem_singleton, and_self,
+        true_and]
+      omega
+  | K1, (Q5, Q10) =>
+    simp [irreducibleSet']
+    have x_isPresent := isPresent_of_isIrreducible h
+    simp only [IsPresent, charges, Finset.product_eq_sprod, Multiset.mem_map, Prod.exists] at x_isPresent
+    simp only [← Multiset.mem_toFinset, Finset.val_toFinset, Finset.mem_product] at x_isPresent
+    obtain ⟨q1, q2, q3, ⟨h1, h2, h3⟩, hsum⟩ := x_isPresent
+    refine ⟨{q1}, {q2, q3}, ⟨?_, ?_⟩, (h _ ?_).mpr ?_⟩
+    · -- membership of Multiset
+      simp [Finset.insert_subset_iff]
+      simp [finsetOfCodimensionOneConfig] at hx
+      rw [Finset.mem_product] at hx
+      obtain ⟨h5, h10⟩ := hx
+      simp at h5 h10
+      exact ⟨h5 h1, h10 h2, h10 h3⟩
+    · -- sum
+      simp
+      omega
+    · -- mem powerset
+      apply subset_of_iff_mem_powerset.mp
+      simp_all [Subset]
+    · -- is present
+      simp only [IsPresent, charges, Finset.product_eq_sprod, Multiset.mem_map, Prod.exists]
+      use q1, q2, q3
+      simp only [Finset.singleton_product, Finset.map_val, Finset.product_val, Finset.insert_val,
+        Finset.singleton_val, Function.Embedding.coeFn_mk, Multiset.mem_map, Prod.mk.injEq, true_and,
+        exists_eq_right,]
+      repeat rw [SProd.sprod, Multiset.instSProd, Multiset.mem_product]
+      simp only [Multiset.toFinset_singleton, Finset.singleton_val, Multiset.mem_singleton,
+        Multiset.insert_eq_cons, Multiset.toFinset_cons, Finset.insert_val, Multiset.mem_ndinsert,
+        true_or, or_true, and_self, true_and]
+      omega
+  | K2, (qHd, qHu, Q10) =>
+    simp [irreducibleSet']
+    have x_isPresent := isPresent_of_isIrreducible h
+    simp only [IsPresent, charges, Finset.product_eq_sprod, Multiset.mem_map, Prod.exists] at x_isPresent
+    simp only [← Multiset.mem_toFinset, Finset.val_toFinset, Finset.mem_product] at x_isPresent
+    obtain ⟨q1, q2, q3, ⟨h1, h2, h3⟩, hsum⟩ := x_isPresent
+    refine ⟨q1, q2, {q3}, ⟨?_, ?_⟩, (h _ ?_).mpr ?_⟩
+    · -- membership of Multiset
+      rw [Option.mem_toFinset, Option.mem_def] at h1 h2
+      subst h1 h2
+      rw [finsetOfCodimensionOneConfig, Finset.product_eq_sprod, Finset.mem_product] at hx
+      simp at hx
+      obtain ⟨ha, hb, hc⟩ := hx
+      simpa [Finset.insert_subset_iff] using ⟨ha, hb, hc h3⟩
+    · -- sum
+      simp
+      omega
+    · -- mem powerset
+      apply subset_of_iff_mem_powerset.mp
+      simp_all [Subset]
+    · -- is present
+      simp only [IsPresent, charges, Finset.product_eq_sprod, Multiset.mem_map, Prod.exists]
+      use q1, q2, q3
+      simp only [Finset.singleton_product, Finset.map_val, Finset.product_val, Finset.insert_val,
+        Finset.singleton_val, Function.Embedding.coeFn_mk, Multiset.mem_map, Prod.mk.injEq, true_and,
+        exists_eq_right]
+      repeat rw [SProd.sprod, Multiset.instSProd, Multiset.mem_product]
+      simp only [Option.toFinset_some, Finset.singleton_val, Multiset.mem_singleton,
+        Multiset.insert_eq_cons, Multiset.toFinset_cons, Multiset.toFinset_singleton,
+        Finset.insert_val, Multiset.mem_ndinsert, true_or, or_true, and_self, true_and]
+      omega
+  | W1, (Q5, Q10) =>
+    simp [irreducibleSet']
+    apply And.intro _ h
+    have x_isPresent := isPresent_of_isIrreducible h
+    simp only [IsPresent, charges, Finset.product_eq_sprod, Multiset.mem_map, Prod.exists] at x_isPresent
+    simp only [← Multiset.mem_toFinset, Finset.val_toFinset, Finset.mem_product] at x_isPresent
+    obtain ⟨q1, q2, q3, q4, ⟨h1, h2, h3, h4⟩, hsum⟩ := x_isPresent
+    refine ⟨{q1}, {q2, q3, q4}, ⟨?_, ?_⟩, (h _ ?_).mpr ?_⟩
+    · -- membership of Multiset
+      simp [Finset.insert_subset_iff]
+      simp [finsetOfCodimensionOneConfig] at hx
+      rw [Finset.mem_product] at hx
+      obtain ⟨h5, h10⟩ := hx
+      simp at h5 h10
+      exact ⟨h5 h1, h10 h2, h10 h3, h10 h4⟩
+    · -- sum
+      simp
+      omega
+    · -- mem powerset
+      apply subset_of_iff_mem_powerset.mp
+      simp_all [Subset]
+    · -- is present
+      simp only [IsPresent, charges, Finset.product_eq_sprod, Multiset.mem_map, Prod.exists]
+      use q1, q2, q3, q4
+      simp only [Finset.singleton_product, Finset.map_val, Finset.product_val, Finset.insert_val,
+        Finset.singleton_val, Function.Embedding.coeFn_mk, Multiset.mem_map, Prod.mk.injEq, true_and,
+        exists_eq_right,]
+      repeat rw [SProd.sprod, Multiset.instSProd, Multiset.mem_product]
+      simp only [Multiset.toFinset_singleton, Finset.singleton_val, Multiset.mem_singleton,
+        Multiset.insert_eq_cons, Multiset.toFinset_cons, Finset.insert_val, Multiset.mem_ndinsert,
+        true_or, or_true, and_self, true_and]
+      omega
+  | W2, (qHd, Q10) =>
+    simp [irreducibleSet']
+    apply And.intro _ h
+    have x_isPresent := isPresent_of_isIrreducible h
+    simp only [IsPresent, charges, Finset.product_eq_sprod, Multiset.mem_map, Prod.exists] at x_isPresent
+    simp only [← Multiset.mem_toFinset, Finset.val_toFinset, Finset.mem_product] at x_isPresent
+    obtain ⟨q1, q2, q3, q4, ⟨h1, h2, h3, h4⟩, hsum⟩ := x_isPresent
+    refine ⟨q1, {q2, q3, q4}, ⟨?_, ?_⟩, (h _ ?_).mpr ?_⟩
+    · -- membership of Multiset
+      rw [Option.mem_toFinset, Option.mem_def] at h1
+      subst h1
+      rw [finsetOfCodimensionOneConfig, Finset.product_eq_sprod, Finset.mem_product] at hx
+      simp at hx
+      obtain ⟨ha, hb⟩ := hx
+      simpa [Finset.insert_subset_iff] using ⟨ha, hb h2, hb h3, hb h4⟩
+    · -- sum
+      simp
+      omega
+    · -- mem powerset
+      apply subset_of_iff_mem_powerset.mp
+      simp_all [Subset]
+    · -- is present
+      simp only [IsPresent, charges, Finset.product_eq_sprod, Multiset.mem_map, Prod.exists]
+      use q1, q2, q3, q4
+      simp only [Finset.singleton_product, Finset.map_val, Finset.product_val, Finset.insert_val,
+        Finset.singleton_val, Function.Embedding.coeFn_mk, Multiset.mem_map, Prod.mk.injEq, true_and,
+        exists_eq_right]
+      repeat rw [SProd.sprod, Multiset.instSProd, Multiset.mem_product]
+      simp only [Option.toFinset_some, Finset.singleton_val, Multiset.mem_singleton,
+        Multiset.insert_eq_cons, Multiset.toFinset_cons, Multiset.toFinset_singleton,
+        Finset.insert_val, Multiset.mem_ndinsert, true_or, or_true, and_self, true_and]
+      omega
+  | W3, (qHu, Q5) =>
+    simp [irreducibleSet']
+    have x_isPresent := isPresent_of_isIrreducible h
+    simp only [IsPresent, charges, Finset.product_eq_sprod, Multiset.mem_map, Prod.exists] at x_isPresent
+    simp only [← Multiset.mem_toFinset, Finset.val_toFinset, Finset.mem_product] at x_isPresent
+    obtain ⟨q1, q2, q3, ⟨h1, h2, h3⟩, hsum⟩ := x_isPresent
+    refine ⟨q1, {q2, q3}, ⟨?_, ?_⟩, (h _ ?_).mpr ?_⟩
+    · -- membership of Multiset
+      rw [Option.mem_toFinset, Option.mem_def] at h1
+      subst h1
+      rw [finsetOfCodimensionOneConfig, Finset.product_eq_sprod, Finset.mem_product] at hx
+      simp at hx
+      obtain ⟨ha, hb⟩ := hx
+      simpa [Finset.insert_subset_iff] using ⟨ha, hb h2, hb h3⟩
+    · -- sum
+      simp
+      omega
+    · -- mem powerset
+      apply subset_of_iff_mem_powerset.mp
+      simp_all [Subset]
+    · -- is present
+      simp only [IsPresent, charges, Finset.product_eq_sprod, Multiset.mem_map, Prod.exists]
+      use q1, q2, q3
+      simp only [Finset.singleton_product, Finset.map_val, Finset.product_val, Finset.insert_val,
+        Finset.singleton_val, Function.Embedding.coeFn_mk, Multiset.mem_map, Prod.mk.injEq, true_and,
+        exists_eq_right]
+      repeat rw [SProd.sprod, Multiset.instSProd, Multiset.mem_product]
+      simp only [Option.toFinset_some, Finset.singleton_val, Multiset.mem_singleton,
+        Multiset.insert_eq_cons, Multiset.toFinset_cons, Multiset.toFinset_singleton,
+        Finset.insert_val, Multiset.mem_ndinsert, true_or, or_true, and_self, true_and]
+      omega
+  | W4, (qHd, qHu, Q5) =>
+    simp [irreducibleSet']
+    have x_isPresent := isPresent_of_isIrreducible h
+    simp only [IsPresent, charges, Finset.product_eq_sprod, Multiset.mem_map, Prod.exists] at x_isPresent
+    simp only [← Multiset.mem_toFinset, Finset.val_toFinset, Finset.mem_product] at x_isPresent
+    obtain ⟨q1, q2, q3, ⟨h1, h2, h3⟩, hsum⟩ := x_isPresent
+    refine ⟨q1, q2, {q3}, ⟨?_, ?_⟩, (h _ ?_).mpr ?_⟩
+    · -- membership of Multiset
+      rw [Option.mem_toFinset, Option.mem_def] at h1 h2
+      subst h1 h2
+      rw [finsetOfCodimensionOneConfig, Finset.product_eq_sprod, Finset.mem_product] at hx
+      simp at hx
+      obtain ⟨ha, hb, hc⟩ := hx
+      simpa [Finset.insert_subset_iff] using ⟨ha, hb, hc h3⟩
+    · -- sum
+      simp
+      omega
+    · -- mem powerset
+      apply subset_of_iff_mem_powerset.mp
+      simp_all [Subset]
+    · -- is present
+      simp only [IsPresent, charges, Finset.product_eq_sprod, Multiset.mem_map, Prod.exists]
+      use q1, q2, q3
+      simp only [Finset.singleton_product, Finset.map_val, Finset.product_val, Finset.insert_val,
+        Finset.singleton_val, Function.Embedding.coeFn_mk, Multiset.mem_map, Prod.mk.injEq, true_and,
+        exists_eq_right]
+      repeat rw [SProd.sprod, Multiset.instSProd, Multiset.mem_product]
+      simp only [Option.toFinset_some, Finset.singleton_val, Multiset.mem_singleton,
+        Multiset.insert_eq_cons, Multiset.toFinset_cons, Multiset.toFinset_singleton,
+        Finset.insert_val, Multiset.mem_ndinsert, true_or, or_true, and_self, true_and]
+      omega
+  | Λ, (Q5, Q10) =>
+    simp [irreducibleSet']
+    have x_isPresent := isPresent_of_isIrreducible h
+    simp only [IsPresent, charges, Finset.product_eq_sprod, Multiset.mem_map, Prod.exists] at x_isPresent
+    simp only [← Multiset.mem_toFinset, Finset.val_toFinset, Finset.mem_product] at x_isPresent
+    obtain ⟨q1, q2, q3, ⟨h1, h2, h3⟩, hsum⟩ := x_isPresent
+    refine ⟨{q1, q2}, {q3}, ⟨?_, ?_⟩, (h _ ?_).mpr ?_⟩
+    · -- membership of Multiset
+      simp [Finset.insert_subset_iff]
+      simp [finsetOfCodimensionOneConfig] at hx
+      rw [Finset.mem_product] at hx
+      obtain ⟨h5, h10⟩ := hx
+      simp at h5 h10
+      exact ⟨⟨h5 h1, h5 h2⟩, h10 h3⟩
+    · -- sum
+      simp
+      omega
+    · -- mem powerset
+      apply subset_of_iff_mem_powerset.mp
+      simp_all [Subset]
+    · -- is present
+      simp only [IsPresent, charges, Finset.product_eq_sprod, Multiset.mem_map, Prod.exists]
+      use q1, q2, q3
+      simp only [Finset.singleton_product, Finset.map_val, Finset.product_val, Finset.insert_val,
+        Finset.singleton_val, Function.Embedding.coeFn_mk, Multiset.mem_map, Prod.mk.injEq, true_and,
+        exists_eq_right,]
+      repeat rw [SProd.sprod, Multiset.instSProd, Multiset.mem_product]
+      simp only [Multiset.toFinset_singleton, Finset.singleton_val, Multiset.mem_singleton,
+        Multiset.insert_eq_cons, Multiset.toFinset_cons, Finset.insert_val, Multiset.mem_ndinsert,
+        true_or, or_true, and_self, true_and]
+      omega
+  | β, (qHu, Q5) =>
+    simp [irreducibleSet']
+    have x_isPresent := isPresent_of_isIrreducible h
+    simp only [IsPresent, charges, Finset.product_eq_sprod, Multiset.mem_map, Prod.exists] at x_isPresent
+    simp only [← Multiset.mem_toFinset, Finset.val_toFinset, Finset.mem_product] at x_isPresent
+    obtain ⟨q1, q2, ⟨h1, h2⟩, hsum⟩ := x_isPresent
+    refine ⟨q1, {q2}, ⟨?_, ?_⟩, (h _ ?_).mpr ?_⟩
+    · -- membership of Multiset
+      rw [Option.mem_toFinset, Option.mem_def] at h1
+      subst h1
+      rw [finsetOfCodimensionOneConfig, Finset.product_eq_sprod, Finset.mem_product] at hx
+      simp at hx
+      obtain ⟨ha, hb⟩ := hx
+      simpa [Finset.insert_subset_iff] using ⟨ha, hb h2⟩
+    · -- sum
+      simp
+      omega
+    · -- mem powerset
+      apply subset_of_iff_mem_powerset.mp
+      simp_all [Subset]
+    · -- is present
+      simp only [IsPresent, charges, Finset.product_eq_sprod, Multiset.mem_map, Prod.exists]
+      use q1, q2
+      simp only [Finset.singleton_product, Finset.map_val, Finset.product_val, Finset.insert_val,
+        Finset.singleton_val, Function.Embedding.coeFn_mk, Multiset.mem_map, Prod.mk.injEq, true_and,
+        exists_eq_right]
+      repeat rw [SProd.sprod, Multiset.instSProd, Multiset.mem_product]
+      simp only [Option.toFinset_some, Finset.singleton_val, Multiset.mem_singleton,
+        Multiset.insert_eq_cons, Multiset.toFinset_cons, Multiset.toFinset_singleton,
+        Finset.insert_val, Multiset.mem_ndinsert, true_or, or_true, and_self, true_and]
+      omega
+  | topYukawa, (qHu, Q10) =>
+    simp [irreducibleSet']
+    have x_isPresent := isPresent_of_isIrreducible h
+    simp only [IsPresent, charges, Finset.product_eq_sprod, Multiset.mem_map, Prod.exists] at x_isPresent
+    simp only [← Multiset.mem_toFinset, Finset.val_toFinset, Finset.mem_product] at x_isPresent
+    obtain ⟨q1, q2, q3, ⟨h1, h2, h3⟩, hsum⟩ := x_isPresent
+    refine ⟨q1, {q2, q3}, ⟨?_, ?_⟩, (h _ ?_).mpr ?_⟩
+    · -- membership of Multiset
+      rw [Option.mem_toFinset, Option.mem_def] at h1
+      subst h1
+      rw [finsetOfCodimensionOneConfig, Finset.product_eq_sprod, Finset.mem_product] at hx
+      simp at hx
+      obtain ⟨ha, hb⟩ := hx
+      simpa [Finset.insert_subset_iff] using ⟨ha, hb h2, hb h3⟩
+    · -- sum
+      simp
+      omega
+    · -- mem powerset
+      apply subset_of_iff_mem_powerset.mp
+      simp_all [Subset]
+    · -- is present
+      simp only [IsPresent, charges, Finset.product_eq_sprod, Multiset.mem_map, Prod.exists]
+      use q1, q2, q3
+      simp only [Finset.singleton_product, Finset.map_val, Finset.product_val, Finset.insert_val,
+        Finset.singleton_val, Function.Embedding.coeFn_mk, Multiset.mem_map, Prod.mk.injEq, true_and,
+        exists_eq_right]
+      repeat rw [SProd.sprod, Multiset.instSProd, Multiset.mem_product]
+      simp only [Option.toFinset_some, Finset.singleton_val, Multiset.mem_singleton,
+        Multiset.insert_eq_cons, Multiset.toFinset_cons, Multiset.toFinset_singleton,
+        Finset.insert_val, Multiset.mem_ndinsert, true_or, or_true, and_self, true_and]
+      omega
+  | bottomYukawa, (qHd, Q5, Q10) =>
+    simp [irreducibleSet']
+    have x_isPresent := isPresent_of_isIrreducible h
+    simp only [IsPresent, charges, Finset.product_eq_sprod, Multiset.mem_map, Prod.exists] at x_isPresent
+    simp only [← Multiset.mem_toFinset, Finset.val_toFinset, Finset.mem_product] at x_isPresent
+    obtain ⟨q1, q2, q3, ⟨h1, h2, h3⟩, hsum⟩ := x_isPresent
+    refine ⟨q1, {q2}, {q3}, ⟨?_, ?_⟩, (h _ ?_).mpr ?_⟩
+    · -- membership of Multiset
+      rw [Option.mem_toFinset, Option.mem_def] at h1
+      subst h1
+      rw [finsetOfCodimensionOneConfig, Finset.product_eq_sprod, Finset.mem_product] at hx
+      simp at hx
+      obtain ⟨ha, hb, hc⟩ := hx
+      simpa [Finset.insert_subset_iff] using ⟨ha, hb h2, hc h3⟩
+    · -- sum
+      simp
+      omega
+    · -- mem powerset
+      apply subset_of_iff_mem_powerset.mp
+      simp_all [Subset]
+    · -- is present
+      simp only [IsPresent, charges, Finset.product_eq_sprod, Multiset.mem_map, Prod.exists]
+      use q1, q2, q3
+      simp only [Finset.singleton_product, Finset.map_val, Finset.product_val, Finset.insert_val,
+        Finset.singleton_val, Function.Embedding.coeFn_mk, Multiset.mem_map, Prod.mk.injEq, true_and,
+        exists_eq_right]
+      repeat rw [SProd.sprod, Multiset.instSProd, Multiset.mem_product]
+      simp only [Option.toFinset_some, Finset.singleton_val, Multiset.mem_singleton,
+        Multiset.insert_eq_cons, Multiset.toFinset_cons, Multiset.toFinset_singleton,
+        Finset.insert_val, Multiset.mem_ndinsert, true_or, or_true, and_self, true_and]
+      omega
+
+/-!
+
+## Completeness
+
+-/
+
+lemma irreducibleElems_eq_irreducibleSet' (I : CodimensionOneConfig) (T : PotentialTerm) :
+    irreducibleElems I T = irreducibleSet' I T := by
+  apply Multiset.eq_of_le_of_card_le
+  · refine (Multiset.le_iff_subset ?_).mpr ?_
+    · exact irreducibleElems_nodup I T
+    refine Multiset.subset_iff.mpr ?_
+    intro x hx
+    apply mem_irreducibleSet'_of_irreducible
+    · exact isIrreducible_of_mem_irreducibleElems x hx
+    · apply irreducibleElems_subset_finsetOfCodimensionOneConfig
+      exact hx
+  · rw [irreducibleSet'_card_eq, irreducibleElems_card_eq]
+
+lemma isIrreducible_iff_mem_irreducibleElems {I : CodimensionOneConfig} {T : PotentialTerm}
+    (x : ChargeProfile T) (hx : x ∈ finsetOfCodimensionOneConfig I T) :
+    IsIrreducible x ↔ x ∈ irreducibleElems I T := by
+  symm
+  constructor
+  · intro h
+    apply isIrreducible_of_mem_irreducibleElems
+    exact h
+  · intro h
+    rw [irreducibleElems_eq_irreducibleSet']
+    apply mem_irreducibleSet'_of_irreducible
+    · exact h
+    · exact hx
+
+end ChargeProfile
+
+end PotentialTerm
+
+end SU5U1
+
+end FTheory
